theories/zoo_std/queue_2__code.v
@@ -1,0 +1,43 @@
+From zoo Require Import
+  prelude.
+From zoo.language Require Import
+  typeclasses
+  notations.
+From zoo_std Require Import
+  queue_2__types.
+From zoo Require Import
+  options.
+
+Definition queue_2_create : val :=
+  fun: <> =>
+    let: "sent" := ‘Node{ (), §Null } in
+    { "sent", "sent" }.
+
+Definition queue_2_is_empty : val :=
+  fun: "t" =>
+    "t".{front} == "t".{sentinel}.
+
+Definition queue_2_push : val :=
+  fun: "t" "v" =>
+    match: ‘Node{ (), §Null } with
+    | Node <> <> as "new_sent" =>
+        match: "t".{sentinel} with
+        | Node <> <> as "sent_r" =>
+            "sent_r" <-{head} "v" ;;
+            "sent_r" <-{tail} "new_sent" ;;
+            "t" <-{sentinel} "new_sent"
+        end
+    end.
+
+Definition queue_2_pop : val :=
+  fun: "t" =>
+    match: "t".{front} with
+    | Node <> <> as "front_r" =>
+        match: "front_r".{tail} with
+        | Null =>
+            §None
+        | Node <> <> as "tail" =>
+            "t" <-{front} "tail" ;;
+            ‘Some( "front_r".{head} )
+        end
+    end.
